Mt/sample.lean
@@ -30,21 +30,6 @@ def spec : Mt.Spec :={
   State
   Reservation
   validate := fun ⟨luft, min_x⟩ ⟨x, y⟩ => x ≥ y + luft ∧ x ≥ min_x
-  reservations_can_be_dropped :=by
-    simp only []
-    intro ⟨env_luft, (env_min_x : Nat)⟩ ⟨luft, (min_x : Nat)⟩ ⟨x, y⟩
-      (h : x ≥ y + (env_luft + luft) ∧ x ≥ Nat.max env_min_x min_x)
-
-    show x ≥ y + env_luft ∧ x ≥ env_min_x
-
-    cases h ; constructor
-    . show x ≥ y + env_luft
-      exact calc
-        y + env_luft ≤ y + (env_luft + luft) :=by simp_arith
-                   _ ≤ x                     :=by assumption
-    . show x ≥ env_min_x
-      rename x ≥ Nat.max env_min_x min_x => h
-      exact (nat_max_le.mp h).left 
 }
 
 open Mt
@@ -134,12 +119,14 @@ theorem thread1_valid : thread1.valid_for_reservation' ReservationInstance.empty
 
   clear luft min_x
   intro ⟨luft, min_x⟩ (py : Nat) min_x_def
-  apply valid_for_reservation_bind (spec :=spec) _ _ _ (λ _ => true) λ _ x => x ≥ py
+  apply valid_for_reservation_bind (spec :=spec) _ _ _ (λ _ => true)
+    λ (r : Reservation) x => x ≥ py ∧ r = IsReservation.empty
   . -- validate `let px = x` knowing min_x = py
     -------------------------------------------
     have min_x_def : min_x = py :=min_x_def
     apply valid_for_reservation_read
     intro ⟨x, y⟩ ⟨env_luft, (env_min_x : Nat)⟩ initial_valid _
+    simp only [and_true]
 
     have : x ≥ y + (env_luft + luft) ∧ x ≥ Nat.max env_min_x min_x :=initial_valid
     show (x ≥ y + env_luft ∧ x ≥ Nat.max env_min_x 0) ∧ x ≥ py
@@ -159,9 +146,10 @@ theorem thread1_valid : thread1.valid_for_reservation' ReservationInstance.empty
       exact (nat_max_le.mp h).right
   
   clear luft min_x min_x_def
-  intro ⟨luft, min_x⟩ (px : Nat) px_gt_py
+  intro ⟨luft, min_x⟩ (px : Nat) ⟨px_gt_py, final_check⟩
 
-  apply valid_for_reservation_assert (spec :=spec)
+  rw [final_check]
+  apply valid_for_reservation_assert (spec :=spec) _ _ _ rfl
   . -- validate `assert px ≥ py`
     ----------------------------
     intros
